%%%%(c)
%%%%(c)  This file is a portion of the source for the textbook
%%%%(c)
%%%%(c)    A First Course in Linear Algebra
%%%%(c)    Copyright 2004 by Robert A. Beezer
%%%%(c)
%%%%(c)  See the file COPYING.txt for copying conditions
%%%%(c)
%%%%(c)
Solving each equation for $y$, we have the equivalent system
\begin{align*}
y &= 5 - x\\
y &= 2x - 3.
\end{align*}
Setting these expressions for $y$ equal, we  have the equation 
$5 - x = 2x - 3$, which quickly leads to
 $x = \frac{8}{3}$.  Substituting for $x$ in the first equation, we have $y = 5 - x = 5 - \frac{8}{3} = \frac{7}{3}$.
Thus, the solution is $x = \frac{8}{3}$, $y = \frac{7}{3}$.