%%%%(c)
%%%%(c)  This file is a portion of the source for the textbook
%%%%(c)
%%%%(c)    A First Course in Linear Algebra
%%%%(c)    Copyright 2004 by Robert A. Beezer
%%%%(c)
%%%%(c)  See the file COPYING.txt for copying conditions
%%%%(c)
%%%%(c)
The given equation 
\begin{align*}
\begin{bmatrix} 7 & 12 & 6\\ 6 & 4 & -2 \end{bmatrix} 
&= 
\alpha\begin{bmatrix} 
1 & 3 & 4 \\
 2 & 1 & -1 
\end{bmatrix} 
+ 
\begin{bmatrix} 
4 & 3 & -6 \\
0 & 1 & 1 
\end{bmatrix}\\
%
&= 
\begin{bmatrix} 
\alpha & 3\alpha & 4\alpha \\ 
2\alpha & \alpha & -\alpha 
\end{bmatrix} 
+ 
\begin{bmatrix} 
4 & 3 & -6 \\ 
0 & 1 & 1 
\end{bmatrix}\\
%
&=
\begin{bmatrix} 
4 + \alpha & 3 + 3\alpha & -6 + 4\alpha \\ 
2\alpha & 1 + \alpha & 1 - \alpha 
\end{bmatrix}
\end{align*}
%
leads to the 6 equations in $\alpha$:
%
\begin{align*}
4 + \alpha &= 7\\
3 + 3\alpha &= 12\\
-6 + 4\alpha &= 6\\
2\alpha &= 6\\
1 + \alpha &= 4\\
1 - \alpha &= -2.
\end{align*}
The only value that solves all 6 equations is $\alpha = 3$, which is the solution to the original matrix equation.
