%%%%(c)
%%%%(c)  This file is a portion of the source for the textbook
%%%%(c)
%%%%(c)    A First Course in Linear Algebra
%%%%(c)    Copyright 2004 by Robert A. Beezer
%%%%(c)
%%%%(c)  See the file COPYING.txt for copying conditions
%%%%(c)
%%%%(c)
The given equation
\begin{align*}
\begin{bmatrix}
2 & 1 \\
1 & -2 \\
2 & 6
\end{bmatrix}
&=
\alpha\begin{bmatrix}
3 & 1 \\
2 & 0 \\
1 & 4
\end{bmatrix}
+
\begin{bmatrix}
4 & 1 \\
3 & 2 \\
0 & 1
\end{bmatrix}
=
\begin{bmatrix}
3\alpha - 4 & \alpha - 1 \\
2\alpha - 3 & -2 \\
\alpha & 4\alpha - 1
\end{bmatrix}
\end{align*}
%
gives a system of six equations in $\alpha$:
%
\begin{align*}
3\alpha - 4 &= 2\\
\alpha - 1 &= 1 \\
2\alpha - 3&= 1\\
-2 &= -2\\
\alpha  &= 2\\
4\alpha - 1 &= 6.
\end{align*}
%
Solving each of these equations, we see that the first three and the fifth all lead to the solution $\alpha = 2$, the fourth equation is true no matter what the value of $\alpha$, but the last equation is only solved by $\alpha = 7/4$.  Thus, the system has no solution, and the original matrix equation also has no solution.
