%%%%(c)
%%%%(c)  This file is a portion of the source for the textbook
%%%%(c)
%%%%(c)    A First Course in Linear Algebra
%%%%(c)    Copyright 2004 by Robert A. Beezer
%%%%(c)
%%%%(c)  See the file COPYING.txt for copying conditions
%%%%(c)
%%%%(c)
\begin{align*}
\zerovector
&=\alpha\vect{u} + -\left(\alpha\vect{u}\right)&&\text{\acronymref{property}{AI}}\\
&=\beta\vect{u} + -\left(\alpha\vect{u}\right)&&\text{Hypothesis}\\
&=\beta\vect{u} + (-1)\left(\alpha\vect{u}\right)&&\text{\acronymref{theorem}{AISM}}\\
&=\beta\vect{u} + \left((-1)\alpha\right)\vect{u}&&\text{\acronymref{property}{SMA}}\\
&=\beta\vect{u} + \left(-\alpha\right)\vect{u}\\
&=\left(\beta-\alpha\right)\vect{u}&&\text{\acronymref{property}{DSA}}\\
\intertext{By hypothesis, $\vect{u}\neq\zerovector$, so \acronymref{theorem}{SMEZV} implies}
0&=\beta-\alpha\\
\alpha&=\beta
\end{align*}
