%%%%(c)
%%%%(c)  This file is a portion of the source for the textbook
%%%%(c)
%%%%(c)    A First Course in Linear Algebra
%%%%(c)    Copyright 2004 by Robert A. Beezer
%%%%(c)
%%%%(c)  See the file COPYING.txt for copying conditions
%%%%(c)
%%%%(c)
We have,
%
\begin{align*}
\zerovector
&=\vect{x}-\vect{x}&&\text{\acronymref{property}{AI}}\\
&=\alpha\vect{x}-\vect{x}&&\text{Hypothesis}\\
&=\alpha\vect{x}-1\vect{x}&&\text{\acronymref{property}{O}}\\
&=(\alpha-1)\vect{x}&&\text{\acronymref{property}{DSA}}
\end{align*}
%
So by \acronymref{theorem}{SMEZV} we conclude that $\alpha-1=0$ or $\vect{x}=\zerovector$.  However, since our hypothesis was \emph{for every} $\vect{x}\in V$, we are left with the first possibility and $\alpha=1$.\par
%
There is one flaw in the proof above, and as stated, the problem is not correct either.  Can you spot the flaw and as a result correct the problem statement?  (Hint: \acronymref{example}{VSS}).